tla/MC_ThreadLocalTablesBarriers.tla
@@ -1,0 +1,3 @@
+----------------------- MODULE MC_ThreadLocalTablesBarriers -----------------------
+EXTENDS ThreadLocalTablesBarriers
+=============================================================================
